proved equivalence of list and queue versions, no more deferredFix

examples/graph/theories/BFSProofs.v
@@ -7,6 +7,13 @@ Require Import Equations.Equations.
 Require Import Crush.
 Require Import Data.Graph.Inductive.Graph.
 Require Import Coq.Bool.Bool.
+Require Import Coq.Lists.SetoidList.
+Require Import Omega.
+Require Import Wellfounded.
+Require Import Coq.Relations.Relation_Operators.
+
+Require Import CoLoR.Util.Relation.Lexico.
+Require Import CoLoR.Util.Relation.SN.
 
 (*Helpers*)
 Definition null {a} (l: list a) :=
@@ -50,6 +57,7 @@ Section Ind.
 Context {a : Type} {b : Type} { gr : Type -> Type -> Type} {Hgraph : Graph.Graph gr} {Hlaw : Graph.LawfulGraph gr}.
 
 Definition state : Type := (gr a b) * list (Graph.Path) * RootPath.RTree.
+  
 
 Definition get_graph (s: state) :=
   match s with
@@ -67,16 +75,18 @@ Definition get_paths (s: state) :=
   end.
 
 Definition vertex_in (g: gr a b) (v: Graph.Node) : bool :=
-  match (Graph.match_ v g) with | (None, _) => true | _ => false end.
+  match (Graph.match_ v g) with | (None, _) => false | _ => true end.
 
 Definition in_graph (g : gr a b) (p: Graph.Path) : bool := 
   match p with
-  | nil => true
+  | nil => false
   | v :: xs => vertex_in g v  end. 
+
+Definition notIn_graph g := fun x => negb (in_graph g x). 
 
 Inductive bfs_step : state -> state -> Prop :=
   | bfs_find: forall g l r (p: Graph.Path) (q' : list Graph.Path) c g' (v : Graph.Node) tl,
-    pop_list l (in_graph g) = p :: q' ->
+    pop_list l (notIn_graph g) = p :: q' ->
     p = v :: tl ->
     Graph.match_ v g = (Some c, g') ->
     bfs_step (g, l, r) (g', q' ++ (List.map (fun x => cons x p) (Graph.suc' c)), r ++ (p :: nil)).
@@ -129,7 +139,9 @@ Proof.
   intros. induction H0. assumption. apply IHmulti. eapply v_step. apply H. assumption.
 Qed.
 
-Definition bfs_measure s := (BinInt.Z.abs_nat(Graph.noNodes (get_graph s))).
+Definition natNodes (g : gr a b) := (BinInt.Z.abs_nat(Graph.noNodes g)).
+
+Definition bfs_measure s := natNodes (get_graph s).
 
 Lemma step_decr_measure: forall s s',
   bfs_step s s' ->
@@ -144,7 +156,7 @@ Qed.
 Definition next_state (s: state) : state :=
   match s with
   | (g, q, r) =>
-    let qnew := pop_list q (in_graph g) in
+    let qnew := pop_list q (notIn_graph g) in
     (*So it is same order as in haskell version*)
     if (null qnew) then s else if (Graph.isEmpty g) then s else
     match qnew with
@@ -162,7 +174,7 @@ Definition next_state (s: state) : state :=
   end.
 
 Definition done (s: state) : bool :=
-  null (pop_list (get_queue s) (in_graph (get_graph s))) || (Graph.isEmpty (get_graph s)).
+  null (pop_list (get_queue s) (notIn_graph (get_graph s))) || (Graph.isEmpty (get_graph s)).
 
 (*Every path we create has at least 1 element (v)*)
 Lemma path_nonempty: forall s v,
@@ -184,7 +196,7 @@ Proof.
   - simpl in H0. destruct H0. inversion H0. destruct H0.
   - inversion H1; subst.
     apply in_app_or in H0. destruct H0. simpl in IHvalid.
-     pose proof (pop_list_split l (in_graph g)). destruct H3 as [l']. destruct H3.
+     pose proof (pop_list_split l (notIn_graph g)). destruct H3 as [l']. destruct H3.
     rewrite H2 in H3. apply IHvalid. rewrite <- H3. apply in_or_app. right.
     simpl. right. assumption. 
     assert (forall l, ~In nil (map (fun x : Node => x :: v0 :: tl) l)). { intros.
@@ -197,14 +209,14 @@ Lemma next_step: forall s v, valid s v -> done s = false -> bfs_step s (next_sta
 Proof.
   intros. destruct s. destruct p as [g q]. simpl. unfold done in H0; simpl in H0.
   rewrite Bool.orb_false_iff in H0. destruct H0. rewrite H0. rewrite H1.
-  destruct (pop_list q (in_graph g)) eqn : Q. inversion H0. 
+  destruct (pop_list q (notIn_graph g)) eqn : Q. inversion H0. 
   simpl in H0. 
   (*prove p = nil case impossible*)
-  destruct p eqn : P. pose proof (pop_list_split q (in_graph g)). destruct H2 as [l'].
+  destruct p eqn : P. pose proof (pop_list_split q (notIn_graph g)). destruct H2 as [l'].
   destruct H2. rewrite Q in H2.  pose proof (queue_path_nonempty (g, q, r) v). 
   apply H4 in H. simpl in H. rewrite <- H2 in H. exfalso. apply H. apply in_or_app. right.
   simpl. left. reflexivity. destruct (match_ n g) eqn : M. assert (Q' := Q).
-  apply pop_split_fst in Q. simpl in Q. unfold vertex_in in Q. rewrite M in Q.
+  apply pop_split_fst in Q. unfold notIn_graph in Q. simpl in Q. unfold vertex_in in Q. rewrite M in Q.
   destruct m. eapply bfs_find. apply Q'. reflexivity. apply M. inversion Q.
 Qed. 
 
@@ -240,7 +252,261 @@ Proof.
   intros. apply bfs_tail_elim. intros. destruct (bool_dec (done s0) true) eqn : ?.
   - apply multi_refl.
   - eapply multi_step. eapply next_step. apply H0. apply not_true; assumption. apply H1.
+Qed.
+
+(*Well formed lexicographic measure - maybe put in own section*)
+
+
+Definition natNodes_lt x y := natNodes x < natNodes y.
+Definition natNodes_eq x y := natNodes x = natNodes y.
+Definition list_length_lt {a} (x y : list a) := length x < length y.
+Definition queue_length_lt  {a} (x y : Queue a) := list_length_lt (toList _ x) (toList _ y).
+
+Definition bf_measure_list := 
+  transp (lex (transp natNodes_lt) natNodes_eq (transp  (@list_length_lt Path))).
+
+Definition bf_measure_queue :=
+  transp (lex (transp natNodes_lt) natNodes_eq (transp (@queue_length_lt Path))).
+
+Definition f_nat_lt {a} (f: a -> nat) x y := f x < f y.
+
+Lemma f_nat_lt_acc: forall {a} (f: a -> nat) x n, f x <= n -> Acc (f_nat_lt f) x.
+Proof.
+  intros. generalize dependent x. induction n; auto.
+  - intros. apply Acc_intro. intros. unfold f_nat_lt in *. omega.
+  - unfold f_nat_lt in *. intros. apply Acc_intro. intros. apply IHn. omega.
+Qed.
+
+Lemma f_nat_lt_wf: forall {a} (f: a -> nat), well_founded (f_nat_lt f).
+Proof.
+  red. intro. intro. intro. eapply f_nat_lt_acc. eauto.
+Qed.
+
+
+Lemma wf_bf_measure_list : WF (transp bf_measure_list).
+Proof.
+  eapply WF_lex.
+  - apply wf_transp_WF. unfold transp. 
+    pose proof (f_nat_lt_wf (natNodes)). unfold f_nat_lt in H. unfold natNodes_lt. apply H.
+  - apply wf_transp_WF. unfold transp.
+    pose proof (f_nat_lt_wf (@length Path)). unfold f_nat_lt in H. unfold natNodes_lt. apply H.
+  - unfold Transitive. intros. unfold natNodes_eq in *. omega.
+  - unfold inclusion. unfold RelUtil.compose. intros.
+    unfold transp in *. unfold natNodes_lt in *. unfold natNodes_eq in *. destruct H. omega.
+Qed.
+
+Lemma well_founded_bf_measure_list: well_founded (bf_measure_list).
+Proof.
+  apply WF_transp_wf. apply wf_bf_measure_list.
+Qed.
+
+Lemma wf_bf_measure_queue : WF (transp bf_measure_queue).
+Proof.
+  eapply WF_lex.
+  - apply wf_transp_WF. unfold transp. 
+    pose proof (f_nat_lt_wf (natNodes)). unfold f_nat_lt in H. unfold natNodes_lt. apply H.
+  - apply wf_transp_WF. unfold transp.
+    pose proof (f_nat_lt_wf (fun x => length (toList Path x))). unfold f_nat_lt in H. unfold queue_length_lt.
+    unfold list_length_lt. apply H.
+  - unfold Transitive. intros. unfold natNodes_eq in *. omega.
+  - unfold inclusion. unfold RelUtil.compose. intros.
+    unfold transp in *. unfold natNodes_lt in *. unfold natNodes_eq in *. destruct H. omega.
+Qed.
+
+Lemma well_founded_bf_measure_queue: well_founded (bf_measure_queue).
+Proof.
+  apply WF_transp_wf. apply wf_bf_measure_queue.
+Qed.
+
+
+Instance need_this_for_equations : WellFounded bf_measure_list.
+Proof.
+  unfold WellFounded. apply well_founded_bf_measure_list.
+Defined.
+
+
+Axiom match_None1: forall (g: gr a b) v g',
+  match_ v g = (None, g') -> Graph.Desc g' (noNodes g) (fun x => vIn g x) (fun x y => eIn g x y).
+
+Axiom match_None2: forall (g: gr a b) v,
+  (exists g', match_ v g = (None, g')) <-> ~vIn g v.
+
+(*should prove this from others ,also may have to change edge thing because of multiple edges*)
+Axiom match_None3: forall (g: gr a b) v g',
+  match_ v g = (None, g') -> noNodes g = noNodes g'.
+
+Lemma match_none_size: forall g v g',
+  match_ v g = (None, g') -> natNodes g = natNodes g'.
+Proof.
+  intros. unfold natNodes. erewrite match_None3. reflexivity. apply H.
 Qed. 
+
+Equations bf_list (x : (gr a b) * (list Path)) : RootPath.RTree by wf x bf_measure_list :=
+  bf_list (g, nil) := nil;
+  bf_list (g, (nil :: q')) := if (isEmpty g) then nil else GHC.Err.patternFailure;
+  bf_list (g, ((v :: t) :: q')) := let p:= v :: t in  if (isEmpty g) then nil else
+      match (match_ v g) as y return ((match_ v g = y) -> _) with
+                        | (Some c, g') => fun H : (match_ v g) = (Some c, g') => p :: (bf_list (g', (q' ++ map (fun x => x :: p)  (suc' c))))
+                        | (None, g') => fun H : (match_ v g) = (None, g') => ( bf_list (g', q'))
+                        end (eq_refl)
+
+  
+.
+Next Obligation.
+unfold bf_measure_list. unfold transp. apply lex1. unfold natNodes_lt. eapply match_decr_size. symmetry. apply H.
+Defined.
+Next Obligation.
+unfold bf_measure_list. unfold transp. apply lex2. unfold natNodes_eq. eapply match_none_size. apply H.
+unfold list_length_lt. simpl. omega.
+Defined.
+
+(*Defn*)
+Print bf_list_unfold.
+Check bf_list_unfold_eq.
+(*could be useful*)
+Check bf_list_elim.
+
+
+
+
+(*NOTE: need to resolve this, working with this for now bc of issue with lazy evaluation vs strict*)
+(*TODO: Add to midable before I resolve the issue with hs-toc-qo*)
+(*only difference is that we check if the queue is empty BEFORE calling queueGet*)
+(*
+Definition bf_strict : Queue Path -> gr a b -> RootPath.RTree :=
+deferredFix2
+  (fun (bf : Queue Path -> gr a b -> list Path) (q : Queue Path) (g : gr a b) =>
+   if queueEmpty q || isEmpty g : bool
+       then nil else 
+   let (p, q') := queueGet q in
+   match p with
+   | nil => patternFailure
+   | v :: _ =>
+        let (m, g') := match_ v g in
+        match m with
+        | Some c => p :: bf (queuePutList (Base.map (fun arg_2__ : Node => arg_2__ :: p) (suc' c)) q') g'
+        | None => bf q' g'
+        end
+   end).
+*)
+
+(*TODO: NOTE: I changed the order ot the arguments to make the proofs MUCH easier (lex requires that
+  graph comes first, and I can use the same well-founded proof for both*)
+(*
+Definition flip {a} {b} (x: a * b) : b * a :=
+  match x with
+  | (y, z) => (z, y)
+  end.
+
+Lemma wf_flip: forall {a b : Type} (f: (a * b) -> (a * b) -> Prop),
+  well_founded f -> well_founded (fun x y => f (flip x) (flip y)).
+Proof.
+  intros. unfold well_founded in *. intros. 
+  apply Acc_intro. intros. specialize (H (flip y) (flip a1)). specialize (H (flip y)).
+*)
+
+Definition bf_strict' :  gr a b -> Queue Path -> RootPath.RTree :=
+deferredFix2
+  (fun (bf : gr a b ->  Queue Path ->  list Path)  (g : gr a b) (q : Queue Path) =>
+   if queueEmpty q || isEmpty g : bool
+       then nil else 
+   let (p, q') := queueGet q in
+   match p with
+   | nil => patternFailure
+   | v :: _ =>
+        let (m, g') := match_ v g in
+        match m with
+        | Some c => p :: bf g' (queuePutList (Base.map (fun arg_2__ : Node => arg_2__ :: p) (suc' c)) q')
+        | None => bf g' q'
+        end
+   end).
+
+
+(*test*)
+Definition bf_list_unfold' := 
+fun x : gr a b * list Path =>
+let (g, l) := x in
+match l with
+| nil => nil
+| p :: l0 =>
+    match p with
+    | nil => fun _ : list Path => if isEmpty g then nil else patternFailure
+    | n :: l1 =>
+        fun l2 : list Path =>
+        if isEmpty g
+        then nil
+        else
+         (let (m, g') as y return (match_ n g = y -> list (list Node)) := match_ n g in
+          match m as m0 return (match_ n g = (m0, g') -> list (list Node)) with
+          | Some c =>
+              fun _ : match_ n g = (Some c, g') =>
+              (n :: l1) :: bf_list (g', l2 ++ map (fun x0 : Node => x0 :: n :: l1) (suc' c))
+          | None => fun _ : match_ n g = (None, g') => bf_list (g', l2)
+          end) eq_refl
+    end l0
+end.
+
+Lemma bf_list_unfold'_equiv: forall x,
+  bf_list_unfold' x = bf_list x.
+Proof.
+  intros. unfold bf_list_unfold'. apply bf_list_elim; try(reflexivity).
+Qed.
+
+Lemma bf_list_equiv: forall (x: (gr a b) * (Queue Path)), 
+  bf_strict'  (fst x) (snd x) = bf_list ((fst x), (toList _ (snd x))).
+Proof.
+  intros. unfold bf_strict'. rewrite <- bf_list_unfold'_equiv. simpl.
+  induction (x) as [y IH] using (well_founded_induction well_founded_bf_measure_queue). 
+  destruct y as [g q]. simpl. unfold deferredFix2 in *. unfold curry in *.
+  rewrite (deferredFix_eq_on _ (fun x => True) ( bf_measure_queue )).
+  - simpl. destruct (toList _ q) eqn : Q.  
+    + simpl. assert (queueEmpty q = true). rewrite toList_queueEmpty. assumption. rewrite H.
+      reflexivity.
+    + simpl. assert (queueEmpty q = false). destruct (queueEmpty q) eqn : ?. rewrite toList_queueEmpty in Heqb0.
+      rewrite Heqb0 in Q. inversion Q. reflexivity. rewrite H. simpl.
+      destruct (isEmpty g) eqn : GE. destruct p; reflexivity.
+      destruct (queueGet q) eqn : QG.
+      pose proof (toList_queueGet _ _ _ _ Q). rewrite QG in H0. simpl in H0. destruct H0; subst.
+      destruct p. reflexivity. destruct (match_ n g) eqn : M. destruct m.
+      * specialize (IH (g0, 
+        queuePutList (Base.map (fun arg_2__ : Node => arg_2__ :: n :: p) (suc' c)) q0)). simpl in IH.
+        rewrite IH. simpl. rewrite <- bf_list_unfold'_equiv. simpl.
+        rewrite toList_queuePutList. reflexivity.
+        unfold bf_measure_queue. unfold transp. apply lex1. unfold natNodes_lt. eapply match_decr_size.
+        symmetry. apply M.
+      * specialize (IH (g0, q0)). rewrite IH. simpl. rewrite <- bf_list_unfold'_equiv. simpl.
+        reflexivity. unfold bf_measure_queue. unfold transp. apply lex2. unfold natNodes_eq.
+        eapply match_none_size. apply M. unfold queue_length_lt. unfold list_length_lt.
+        rewrite Q. simpl. omega.
+  -  eapply well_founded_bf_measure_queue.
+  - unfold recurses_on. intros. unfold uncurry. destruct x. destruct (queueEmpty q0) eqn : ?.
+    reflexivity. destruct (isEmpty g1) eqn : ?. reflexivity. simpl. destruct (queueGet q0) eqn : ?.
+    destruct p. reflexivity. destruct (match_ n g1) eqn : ?. destruct m.
+    rewrite H0. reflexivity. apply I. unfold bf_measure_queue. unfold transp. apply lex1.
+    unfold natNodes_lt. eapply match_decr_size. symmetry. apply Heqd. apply H0. apply I.
+    unfold bf_measure_queue. unfold transp. apply lex2. unfold natNodes_eq. eapply match_none_size.
+    apply Heqd. unfold queue_length_lt. unfold list_length_lt. 
+    destruct (toList Path q0) eqn : ?. rewrite <- toList_queueEmpty in Heql. rewrite Heql in Heqb0.
+    inversion Heqb0. eapply toList_queueGet in Heql. rewrite Heqp in Heql. simpl in Heql. destruct Heql; subst.
+    simpl. omega.
+  - apply I.
+Qed.
+
+(*Finally, the result we want (mostly - TODO NEED to figure out order stuff*)
+Lemma bf_list_equiv': forall (g: gr a b) (q: Queue Path),
+  bf_strict' g q = bf_list (g,(toList _ q)).
+Proof.
+  intros. pose proof (bf_list_equiv (g, q)). simpl in H. assumption.
+Qed. 
+
+(*Equivalence*)
+
+(*Steps:
+1. show we can unwrap BFS if first in queue not in graph
+2. show we can unwrap to pop_list
+3. equivalence of lists and queues
+4. then can unwarp deferredFix and prove termination
+5. need something about the paths, tail vs regular recursive*)
 
 (*Next step: try to prove this is equivalent to Haskell BFS, then can just work with this version/ valid states*)
 End Ind.
